Refinement with preconditions, including intro rules.
Signed-off-by: David Cock <david.cock@inf.ethz.ch>

Refine_Mod2.thy
@@ -16,14 +16,54 @@ theory Refine_Mod2
   imports Refinements
 begin
 
-definition sr_mod_2 :: "(nat \<times> nat) set"
-  where "sr_mod_2 = {(m,n). m mod 2 = n mod 2}"
+definition lift_mod_2 :: "nat \<Rightarrow> nat"
+  where "lift_mod_2 = (\<lambda>n. n mod 2)"
 
-definition fr_id :: "(nat \<times> nat) set"
-  where "fr_id = {(m,n). m = n}"
+lemma add_refines:
+  "((\<Gamma>a,UNIV,Language.Basic id), (\<Gamma>c,UNIV,Language.Basic (\<lambda>n. n + 2)))
+      \<in> refinement_s (separable_lift lift_mod_2 id)"
+  unfolding lift_mod_2_def by(auto intro: refinement_s_BasicI)
 
-lemma
-  "(Language.Basic id, Language.Basic (\<lambda>x. x + 2)) \<in> refinement_s (separable_sr sr_mod_2 fr_id) \<Gamma>a \<Gamma>c"
-  unfolding sr_mod_2_def by(auto intro:refinement_s_BasicI)
+lemma double_refines:
+  "((\<Gamma>a,UNIV,Language.Basic (\<lambda>n. 0)), (\<Gamma>c,UNIV,Language.Basic (\<lambda>n. n * 2)))
+      \<in> refinement_s (separable_lift lift_mod_2 id)"
+  unfolding lift_mod_2_def by(auto intro: refinement_s_BasicI)
+
+lemma halve_refines:
+  "((\<Gamma>a,UNIV,Language.Basic (\<lambda>n. n + 1)),
+    (\<Gamma>c,Semantic.Normal ` {n. n mod 4 = 2},Language.Basic (\<lambda>n. n div 2)))
+      \<in> refinement_s (separable_lift lift_mod_2 id)"
+  unfolding lift_mod_2_def
+proof(rule refinement_s_BasicI, auto) (* XXX - not the way to do it. *)
+  (* But here you're down to the object logic. *) 
+  fix n::nat
+  assume mod_4_2: "n mod 4 = 2"
+  have "n = 4 * (n div 4) + (n mod 4)"
+    by(simp)
+  also from mod_4_2 have "... = 4 * (n div 4) + 2"
+    by(simp)
+  also have "... = (2 * (2 * (n div 4))) + 2"
+    by(simp)
+  finally have n_sum: "n = 2 * (2 * (n div 4)) + 2" .
+  hence "n div 2 = ((2 * (2 * (n div 4))) + 2) div 2"
+    by(simp)
+  also have "... = (2 * (n div 4)) + (2 div 2)"
+    by(simp)
+  also have "... = 2 * (n div 4) + 1"
+    by(simp)
+  finally have "n div 2 mod 2 = (2 * (n div 4) + 1) mod 2"
+    by(simp)
+  also have "... = 1"
+    by(simp)
+  also {
+    from n_sum have "n mod 2 = (2 * (2 * (n div 4)) + 2) mod 2"
+      by(simp)
+    also have "... = 0" by(simp)
+    finally have "1 = Suc (n mod 2)" by(simp)
+  }
+  finally show "n div 2 mod 2 = Suc (n mod 2)" .
+qed
+
+(* XXX - SeqI needs to take a concrete hoare triple. *)
 
 end
